updating

noActionStacksInIVars/rollbackWellFormed.v
@@ -12,41 +12,9 @@ Require Import hetList.
 Require Import Coq.Program.Equality. 
 Require Import Heap. 
 Require Import Coq.Sets.Powerset_facts. 
- 
-Ltac eqIn H := unfoldTac; 
-  match type of H with
-      |forall x, Ensembles.In ?X (Union ?X ?T (Singleton ?X ?t)) x -> ?y =>
-       assert(Ensembles.In X(Union X T (Singleton X t)) t) by 
-           (apply Union_intror; constructor)
-  end.
+Require Import IndependenceCommon. 
 
-Axiom uniqueTP : forall T1 T2 t, tIn (tUnion T1 T2) t -> tIn T1 t -> tIn T2 t -> False. 
-
-Theorem UnionEqTID : forall T T' tid s1 s2 M s1' s2' M',
-                       tUnion T (tSingleton(tid,s1,s2,M)) = tUnion T' (tSingleton(tid,s1',s2',M')) ->
-                       T = T' /\ s1 = s1' /\ s2 = s2' /\ M = M'. 
-Proof. 
-  intros. unfoldSetEq H. assert(tIn (tUnion T (tSingleton(tid,s1,s2,M)))(tid,s1,s2,M)). 
-  apply Union_intror. constructor. copy H.  apply H0 in H. inversion H.  
-  {assert(thread_lookup (tUnion T' (tSingleton(tid,s1',s2',M'))) tid (tid,s1,s2,M)). 
-   econstructor. econstructor. eauto. auto. 
-   assert(thread_lookup (tUnion T' (tSingleton(tid,s1',s2',M'))) tid (tid,s1',s2',M')). 
-   econstructor. apply Union_intror. constructor. auto. eapply uniqueThreadPool in H5; eauto. 
-   inv H5. repeat constructor; auto. eqSets. 
-   {assert(tIn (tUnion T (tSingleton(tid,s1,s2,M))) x). constructor. auto. copy H5. apply H0 in H5. 
-    inversion H5; subst. auto. inv H8. exfalso. eapply uniqueTP; eauto. constructor. }
-   {assert(tIn (tUnion T' (tSingleton(tid,s1,s2,M))) x). constructor. auto. copy H5. 
-    apply H1 in H5. inversion H5; subst. auto. inv H8. exfalso. eapply uniqueTP; eauto. 
-    constructor. }
-  }
-  {subst. inv H3. repeat constructor; auto. eqSets. 
-   {assert(tIn (tUnion T (tSingleton(tid,s1,s2,M))) x). constructor. auto. copy H4. apply H0 in H4. 
-    inversion H4; subst. auto. inv H6. exfalso. eapply uniqueTP; eauto. constructor. }
-   {assert(tIn (tUnion T' (tSingleton(tid,s1,s2,M))) x). constructor. auto. copy H4. 
-    apply H1 in H4. inversion H4; subst. auto. inv H6. exfalso. eapply uniqueTP; eauto. 
-    constructor. }
-  }
-Qed. 
+Hint Constructors actionTerm. 
 
 Definition commitPool' T := forall tid s1 s2 M, tIn T (tid,s1,s2,M) -> 
                                                 s1 = unlocked nil \/ exists N, s1 = specStack nil N.
@@ -56,84 +24,222 @@ Proof.
   intros. unfold commitPool'. intros. unfoldSetEq H. apply H1 in H0. inv H0.
   inv H3; try solve[inv H4; eauto]. 
 Qed. 
-
-(*
-Theorem passThroughAct : forall a M M' T s1 s2 H H' tid,
-        actionTerm a M' -> unspecHeap H H' ->
-        spec_multistep H' (tUnion (unspecPoolAux T) (unspecPoolAux (tSingleton(tid,a::s1,s2,M))))
-                       H (tUnion T (tSingleton(tid,a::s1,s2,M))) ->
-        exists T'' H'', 
-          spec_multistep H' (tUnion (unspecPoolAux T) (unspecPoolAux (tSingleton(tid,a::s1,s2,M))))
-                         H'' (tUnion T'' (tSingleton(tid,s1,s2,M'))) /\
-          spec_multistep H'' (tUnion T'' (tSingleton(tid,s1,s2,M')))
-                         H (tUnion T (tSingleton(tid,s1,s2,M'))). 
-Proof.
-  intros. dependent induction H2.  
-  {rewrite <- unspecUnionComm in x. symmetry in x. apply eqUnspec in x. unfold commitPool in x. 
-   assert(tIn (tUnion T (tSingleton(tid,a::s1,s2,M))) (tid,a::s1,s2,M)). apply Union_intror. 
-   constructor. apply x in H. inv H. }
-  {copy H. apply specStepSingleton in H. invertHyp. unfoldSetEq x. eqIn H.
-   apply H in H5. inversion H5; subst. 
-   {admit. }
-   {inv H6. inv H7. inv H10. inv H6. erewrite unspecSingleton; eauto. 
-Admitted. 
-*)
-
-Inductive eraseTrm : list action -> trm -> trm -> Prop :=
-|eraseTrmNil : forall M, eraseTrm nil M M
-|eraseTrmRead : forall x t E d s M, eraseTrm (s++[rAct x t E d]) M t
-|eraseTrmWrite : forall x t E M d N s, eraseTrm (s++[wAct x t E M d]) N t
-|eraseTrmNew : forall x t E d s M, eraseTrm (s++[nAct t E d x]) M t
-|eraseTrmFork : forall t E M d N s n, eraseTrm (s++[fAct t E M d n]) N t
-|eraseTrmSR : forall t E M N d M' s, eraseTrm (s++[srAct t E M N d]) M' t. 
-
-Theorem unspecEraseTrm : forall tid s1 s2 M M', 
-                          eraseTrm s1 M M' ->
-                          unspecThread(tid,unlocked s1,s2,M) (tSingleton(tid,unlocked nil,s2,M')). 
-Proof.
-  intros. destructLast s1. 
-  {inv H; try invertListNeq. auto. }
-  {invertHyp. destruct x; inv H; try solve[invertListNeq]; apply lastElementEq in H1; 
-   inv H1; unspecThreadTac; auto. }
-Qed. 
-
-Theorem eEraseTrm : forall s1 M, exists M', eraseTrm s1 M M'. 
-  intros. destructLast s1. 
-  {econstructor. econstructor. }
-  {invertHyp. destruct x; econstructor; econstructor. }
-Qed. 
-
-Ltac eraseTrmTac s1 M := assert(exists M', eraseTrm s1 M M') by apply eEraseTrm; invertHyp.            
-
-Definition notIn T tid := ~(exists t, thread_lookup T tid t). 
-
-Theorem passThroughAct : forall a M M' T T' s1 s2 H H' tid,
-        actionTerm a M' -> notIn T tid ->
-        spec_multistep H T H' (tUnion T' (tSingleton(tid,locked(a::s1),s2,M))) ->
-        exists T'' H'', 
-          spec_multistep H T H'' (tUnion T'' (tSingleton(tid,locked s1,s2,M'))) /\
-          spec_multistep H'' (tUnion T'' (tSingleton(tid,locked s1,s2,M')))
-                         H' (tUnion T' (tSingleton(tid,locked(a::s1),s2,M))). 
-Proof. 
-  intros. dependent induction H2. 
-  {unfold notIn in H1. exfalso. apply H1. econstructor. econstructor. 
-   apply Union_intror. constructor. auto. }
-  {
-
-
-Theorem passThroughAct' : forall a M M' T T' s1 s2 H H' tid,
-        actionTerm a M' -> 
-        spec_multistep H (tUnion T(tSingleton(tid,unlocked nil,s2,M)))
-                       H' (tUnion T' (tSingleton(tid,locked(a::s1),s2,M))) ->
-        exists T'' H'', 
-          spec_multistep H T H'' (tUnion T'' (tSingleton(tid,locked s1,s2,M'))) /\
-          spec_multistep H'' (tUnion T'' (tSingleton(tid,locked s1,s2,M')))
-                         H' (tUnion T' (tSingleton(tid,locked(a::s1),s2,M))). 
-Proof. 
-  intros. 
-
-Hint Constructors actionTerm.
  
+Theorem eraseTrmConsSame : forall a l M' M'' N,
+                             actionTerm a M' -> 
+                             eraseTrm l M' M'' -> eraseTrm (a::l) N M''. 
+Proof.
+  intros. destructLast l. 
+  {rewrite <- (app_nil_l [a]). inv H; inv H0; try invertListNeq; constructor. }
+  {invertHyp. destruct x; inv H0; try solve[invertListNeq]; apply lastElementEq in H2; 
+   try solveByInv; inv H2; rewrite app_comm_cons; constructor. }
+Qed. 
+
+Inductive spec_multistep_rev : sHeap -> pool -> sHeap -> pool -> Prop :=
+    smulti_refl_r : forall (h : sHeap) (p2 : pool), spec_multistep_rev h p2 h p2
+  | smulti_step_r : forall (T T' t' t'' : pool) (h h' h'' : sHeap),
+                  spec_multistep_rev h T h' (tUnion T' t') ->
+                  spec_step h' T' t' h'' T' t'' ->
+                  spec_multistep_rev h T h'' (tUnion T' t''). 
+
+Theorem spec_multi_rev_trans : forall H T H' T' H'' T'',
+                              spec_multistep_rev H T H' T' ->
+                              spec_multistep_rev H' T' H'' T'' ->
+                              spec_multistep_rev H T H'' T''.
+Proof. 
+  intros. induction H1. 
+  {auto. } 
+  {econstructor. Focus 2. eassumption. eapply IHspec_multistep_rev. eauto. }
+Qed. 
+
+Theorem smultiSmultiRevEq : forall H T H' T',
+                            spec_multistep H T H' T' <-> spec_multistep_rev H T H' T'. 
+Proof.
+  intros. split; intros. 
+  {induction H0. 
+   {constructor. }
+   {eapply spec_multi_rev_trans. eapply smulti_step_r. Focus 2. eauto. constructor. 
+    eauto. }
+  }
+  {induction H0. 
+   {constructor. }
+   {eapply spec_multi_trans. eassumption. econstructor; eauto. 
+    constructor. }
+  }
+Qed. 
+
+Inductive rbTerm : list action -> trm -> trm -> Prop :=
+|rbCons : forall a b M M', actionTerm a M' -> rbTerm (a::b) M M'
+|rbNil : forall M M', rbTerm nil M M'.
+
+Inductive rbTerm' : actionStack -> trm -> trm -> Prop :=
+|rbU : forall s M M', rbTerm s M M' -> rbTerm' (unlocked s) M M' 
+|rbL : forall s M M', rbTerm s M M' -> rbTerm' (locked s) M M'
+|rbS : forall s M M' N, rbTerm s M M' -> rbTerm' (specStack s N) M M'. 
+
+Require Import Coq.Logic.Classical_Prop. 
+
+Theorem specStepCouple : forall H tid s1 s2 M H' T t',
+     spec_step H T (tSingleton(tid,s1,s2,M)) H' T t' ->
+     (exists s1' M', t' = tSingleton(tid,s1',s2,M')) \/
+     (exists n N s1' M',t' = tCouple(tid,s1',s2,M') (n::tid,locked nil,nil,N)). 
+Proof.
+  intros. inv H0; unfoldTac; invertHyp; invThreadEq; eauto. 
+  {right. repeat econstructor. }
+  {right. repeat econstructor. }
+Qed. 
+
+Ltac cleanup := 
+  match goal with
+      |H:?x = ?x |- _ => clear H; try cleanup
+  end.  
+
+Theorem passThroughAct : forall a M M' T s1 s2 H H' tid,
+        actionTerm a M' ->
+        spec_multistep_rev H (unspecPoolAux(tUnion T(tSingleton(tid,aCons a s1,s2,M))))
+                       H' (tUnion T(tSingleton(tid,aCons a s1,s2,M))) ->
+        exists H'' T'', 
+          spec_multistep_rev H (unspecPoolAux(tUnion T(tSingleton(tid,s1,s2,M'))))
+                       H'' (tUnion T'' (tSingleton(tid,s1,s2,M'))) /\
+          spec_multistep_rev H'' (tUnion T'' (tSingleton(tid,s1,s2,M')))
+                         H (tUnion T(tSingleton(tid,s1,s2,M'))). 
+Proof.  
+  Admitted. 
+
+Ltac takeTStepRev :=
+  match goal with
+  | H:Ensembles.In thread ?T ?t
+    |- _ =>
+        apply pullOut in H; rewrite H; unfoldTac; rewrite UnionSwap;
+         econstructor
+  end.
+
+Theorem aConsEq : forall a b c d, aCons a b = aCons c d -> a = c /\ b = d. 
+Proof.
+  intros. destruct b; destruct d; simpl in *; inv H; auto.
+Qed. 
+
+Theorem eraseTrmConsSame' : forall a M' N s1 s2 tid,
+                             actionTerm a M' -> 
+                             unspecPoolAux(tSingleton(tid,s1,s2,M')) = 
+                             unspecPoolAux(tSingleton(tid,aCons a s1,s2,N)). 
+Proof.
+  intros. destruct s1. 
+  {simpl. repeat erewrite unspecSingleton; eauto. }
+  {destructLast l. 
+   {simpl. erewrite unspecSingleton; eauto. erewrite unspecSingleton; eauto. 
+    inv H; unspecThreadTac; rewrite app_nil_l; auto.  }
+   {invertHyp. assert(exists t', unspecThread (tid,unlocked(x0++[x]),s2,M') t'). 
+    apply unspecThreadTotal. invertHyp. erewrite unspecSingleton; eauto. 
+    erewrite unspecSingleton; eauto. inv H1; try solve[invertListNeq]; inv H6; 
+    apply lastElementEq in H1; subst; simpl; rewrite app_comm_cons; unspecThreadTac; auto. }
+  }
+  {simpl. repeat erewrite unspecSingleton; eauto. }
+Qed. 
+
+Theorem unspecSpecSame : forall a M' N s1 s2 tid,
+                             unspecPoolAux(tSingleton(tid,aCons a s1,s2,M')) = 
+                             unspecPoolAux(tSingleton(tid,aCons a s1,s2,N)). 
+Proof.
+  intros. destruct s1. 
+  {simpl. repeat erewrite unspecSingleton; eauto. }
+  {destructLast l. 
+   {Admitted. 
+
+Theorem specStepExistsIn : forall H T t H' t',
+                             spec_step H T t H' T t' ->
+                             exists x, tIn t' x. 
+Proof.
+  intros. inv H0; repeat econstructor. 
+Qed. 
+  
+Require Import Coq.Logic.Classical_Prop.
+ 
+Ltac exMid a b := let n := fresh
+                  in (assert(n:a=b\/a<>b) by apply classic); inv n. 
+
+
+Theorem UnionSubtract : forall U A x,
+                          Ensembles.In U A x ->
+                          A = Union U (Subtract U A x) (Singleton U x). 
+Proof.
+  intros. eqSets. 
+  {assert(x=x0\/x<>x0). apply classic. inv H1. solveSet. constructor. 
+   constructor. auto. intros c. inv c. apply H2; auto. }
+  {inv H0. inv H1. auto. inv H1. auto. }
+Qed. 
+
+Ltac stacksNeq := 
+  match goal with
+      |H:aCons ?a ?b = aCons ?c ?d |- _ => 
+       let n1 := fresh
+       in let n2 := fresh
+          in apply aConsEq in H; inversion H as [n1 n2]; inv n1
+  end.
+
+Theorem passThroughWrite : forall M M' T T' s1 sc s2 H H' tid x E N' d,
+        heap_lookup x H' = Some (sfull sc [] SPEC tid N') -> 
+        spec_multistep_rev H (tUnion T(unspecPoolAux(tSingleton(tid,aCons (wAct x M' E N' d) s1,s2,M))))
+                       H' (tUnion T'(tSingleton(tid,aCons (wAct x M' E N' d) s1,s2,M))) ->
+          spec_multistep_rev H (tUnion T(unspecPoolAux(tSingleton(tid,s1,s2,M'))))
+                             (replace x (sempty sc) H') (tUnion T'(tSingleton(tid,s1,s2,M'))). 
+Proof.
+  intros. dependent induction H1. 
+  {admit. }
+  {inv H. 
+   {exMid tid tid0. 
+    {apply UnionEqTID in x. invertHyp. eapply IHspec_multistep_rev. Focus 3. 
+     auto. Focus 3. auto. eauto. erewrite unspecSpecSame. eauto. }
+    {copy x. unfoldSetEq x. eqIn H5. inv H7. takeTStep. Focus 2. eapply SBasicStep; eauto.
+     unfoldTac. rewrite <- UnionSwap. eapply IHspec_multistep_rev; eauto. proveUnionEq H. 
+     rewrite H9. solveSet. inv H9. exfalso. apply H4; auto. }
+   }
+   {copy x. unfoldSetEq x. eqIn H3. inv H4. symmetry in H. apply UnionSingletonCoupleEq in H; eauto. 
+    rewrite H. unfoldTac. rewrite UnionSwap. econstructor. Focus 2. eapply SFork; eauto. 
+    unfoldTac. rewrite UnionSwap. eapply IHspec_multistep_rev; eauto. rewrite UnionSwap. 
+    rewrite <- UnionSubtract; auto. inv H5. apply aConsEq in H8. invertHyp. solveByInv. 
+    destruct s1; simpl in *; inv H8. }
+   {exMid tid TID. apply UnionEqTID in x. invertHyp. stacksNeq. copy x. unfoldSetEq H. 
+    eqIn H4. inv H. 
+    {varsEq x1 x0. erewrite HeapLookupReplace in H0; eauto. inv H0. takeTStep. Focus 2. 
+     eapply SGet with(h:=replace x0 (sempty sc) h'). rewrite lookupReplaceNeq; eauto.
+     rewrite lookupReplaceSwitch; auto. unfoldTac. rewrite UnionSwap. 
+     eapply IHspec_multistep_rev; eauto. rewrite lookupReplaceNeq in H0; eauto. 
+     proveUnionEq x. rewrite H6. solveSet. }
+    {inv H6. stacksNeq. }
+   }
+   {copy x. unfoldSetEq H. eqIn H3. inv H. 
+    {varsEq x1 x0. 
+     {erewrite HeapLookupReplace in H0; eauto. inv H0. apply UnionEqTID in x. 
+      invertHyp. stacksNeq. rewrite replaceOverwrite. erewrite <- eraseTrmConsSame' in H1; eauto. 
+      rewrite replaceSame; eauto. }
+     {takeTStepRev. Focus 2. eapply SPut with(h:=replace x0 (sempty sc) h'); eauto. 
+      rewrite lookupReplaceNeq; eauto. rewrite lookupReplaceSwitch; eauto. unfoldTac. 
+      rewrite UnionSwap. eapply IHspec_multistep_rev; eauto. rewrite lookupReplaceNeq in H0; eauto. 
+      proveUnionEq x. rewrite H5. solveSet. }
+    }
+    {inv H5. stacksNeq. erewrite <- eraseTrmConsSame' in H1; eauto. rewrite replaceOverwrite. 
+     rewrite replaceSame; eauto. apply UnionEqTID in x. invertHyp. assumption.
+     erewrite HeapLookupReplace in H0; eauto. inv H0. eauto. }
+   }
+   {exMid tid tid0. apply UnionEqTID in x. invertHyp. stacksNeq. copy x. unfoldSetEq H. 
+    eqIn H3. inv H. 
+    {varsEq x1 x0. erewrite lookupExtend in H0. inv H0. takeTStep. Focus 2. 
+     eapply SNew with(h:=replace x0 (sempty sc) h'). erewrite extendReplaceSwitch; eauto. 
+     erewrite lookupExtendNeq in H0; eauto. unfoldTac. rewrite UnionSwap. 
+     eapply IHspec_multistep_rev; eauto. erewrite lookupExtendNeq in H0; eauto. 
+     proveUnionEq x. rewrite H5. solveSet. }
+    {inv H5. stacksNeq. }
+   }
+   {copy x. unfoldSetEq x. eqIn H3. inv H4. symmetry in H. apply UnionSingletonCoupleEq in H. 
+    rewrite H. unfoldTac. rewrite UnionSwap. econstructor. Focus 2. eapply SSpec; eauto. 
+    unfoldTac. rewrite UnionSwap. eapply IHspec_multistep_rev; eauto. rewrite UnionSwap. 
+    rewrite <- UnionSubtract. auto. auto. auto. inv H5. stacksNeq. destruct s1; simpl in*; inv H8. }
+  }
+  Grab Existential Variables. rewrite lookupReplaceNeq. eauto. auto. 
+Qed. 
+
+
 Theorem rollbackWF : forall H H' T TR TR' tidR acts,
                        wellFormed H (tUnion T TR) ->
                        rollback tidR acts H TR H' TR' ->
@@ -142,23 +248,19 @@ Proof.
   intros. induction H1. 
   {auto. }
   {subst. inv H0. inv H1. apply IHrollback. unfoldTac. 
-   econstructor; eauto. repeat rewrite unspecUnionComm in *. destruct s1'. 
-   {admit. }
-   {destructLast l. 
-    {erewrite unspecSingleton; eauto. erewrite unspecSingleton in H3; eauto.
-     Focus 2. simpl. unspecThreadTac. rewrite app_nil_l; auto. simpl in *. 
-     admit. }
-    {invertHyp. eraseTrmTac x. erewrite unspecSingleton; eauto. erewrite unspecSingleton in H3; eauto.
-     Focus 2. simpl. unspecThreadTac. rewrite app_nil_l; auto. simpl in *. 
-     admit. }
-    {
-
-
-
-
-
-
-
-
+   econstructor; eauto. 
+   erewrite unspecHeapRBRead; eauto. rewrite <- Union_associative in H4. 
+   copy H4. rewrite smultiSmultiRevEq in H4. eapply passThroughAct in H4. 
+   Focus 2. constructor. invertHyp. admit. }
+  {subst. inv H0. inv H3. admit. }
+  {subst. inv H0. inv H2. apply IHrollback. unfoldTac. econstructor; eauto. 
+   erewrite unspecHeapRBWrite; eauto. rewrite <- Union_associative in H4. 
+   copy H4. rewrite smultiSmultiRevEq in H4. erewrite unspecUnionComm in H4. 
+   eapply passThroughWrite in H4; eauto. repeat rewrite <- Union_associative. 
+   rewrite smultiSmultiRevEq. rewrite unspecUnionComm. eauto. }
+  {subst. inv H0. inv H3. apply IHrollback. unfoldTac. econstructor; eauto. 
+   erewrite <- unspecHeapRBNew; eauto. rewrite <- Union_associative in H5. 
+   copy H5. rewrite smultiSmultiRevEq in H5. erewrite unspecUnionComm in H5. 
+   
 
 
